Update wording to make the RSAEncryption math clearer

src/extern/dotnet/RSAEncryption.cs
@@ -74,11 +74,6 @@ namespace RSAEncryption {
             }
         }
 
-        public static BigInteger GetPublicModulusFromRSAPublicKey(byteseq publicKey) {
-            RsaKeyParameters publicKeyParam = (RsaKeyParameters) GetPublicKeyFromByteSeq(publicKey);
-            return publicKeyParam.Modulus;
-        }
-
         public static void GenerateKeyPair(int strength, PaddingMode padding, out byteseq publicKey, out byteseq privateKey) {
                 RsaKeyPairGenerator keygen = new RsaKeyPairGenerator();
                 SecureRandom secureRandom = new SecureRandom();
