src/Crypto/RSAEncryption.dfy
@@ -6,8 +6,11 @@ module {:extern "RSAEncryption"} RSAEncryption {
 
     datatype {:extern "PaddingMode"} PaddingMode = PKCS1 | OAEP_SHA1 | OAEP_SHA256 | OAEP_SHA384 | OAEP_SHA512
 
-    // The smallest allowed bit lenght represents PKCS1, where modulus octets >= 11, which implies 11 * 8 - 7 = min bits
-    newtype {:nativeType "int"} BitLength = x | 81 <= x < (0x8000_0000) witness 81
+    // The smallest ciphertext length is defined using PKCS1, where mLen <= k - 11. If mLen == 0 ==> k >= 11
+    // k represents the octet of the modulus, so the min value of k (in bits) is (strength + 7) / 8 == 11 ==> 81
+    // In practice, this number should realistically be 1024 or, more likely, 2048.
+    // TODO: Determine if we want to enforce a min value of 2048 (requires updating the SDK specifications)
+    newtype {:nativeType "int"} Strength = x | 81 <= x < (0x8000_0000) witness 81
 
     // Represents the length in bytes of the hash function output
     const SHA1_HASH_BYTES := 20
@@ -16,16 +19,16 @@ module {:extern "RSAEncryption"} RSAEncryption {
     const SHA512_HASH_BYTES := 64
 
     // GetOctet converts the given number of bits to the octet (byte) size that includes all bits
-    function method GetOctet(bits : BitLength) : nat {
-      (bits as nat + 7) / 8
+    function method GetOctet(bits : nat) : nat {
+      (bits + 7) / 8
     }
 
-    // MinModulusOctets represents the minimum RSA public modulus octets that is usable for a given padding mode
+    // MinModulusOctets represents the minimum RSA public modulus octets (k) that is usable for a given padding mode
     function method MinModulusOctets(padding : PaddingMode) : nat {
       match padding {
-        // 0 = minOctets - 11 ==> minOctets = 11
+        // 0 = k - 11 ==> k = 11
         case PKCS1 => 11
-        // 0 = minOctets - 2 * hashLengthBytes - 2 ==> minModulus = 2 + 2 * hashLengthBytes
+        // 0 = k - 2 * hashLengthBytes - 2 ==> k = 2 + 2 * hashLengthBytes
         case OAEP_SHA1 => 2 * SHA1_HASH_BYTES + 2
         case OAEP_SHA256 => 2 * SHA256_HASH_BYTES + 2
         case OAEP_SHA384 => 2 * SHA384_HASH_BYTES + 2
@@ -33,26 +36,26 @@ module {:extern "RSAEncryption"} RSAEncryption {
         }
     }
 
-    // MaxEncryptionBytes represents the maximum size (in bytes) that plaintextData can be for a given BitLength and
+    // MaxEncryptionBytes represents the maximum size (in bytes) that plaintextData can be for a given modulus n and
     // padding mode
-    function method MaxEncryptionBytes(padding : PaddingMode, n : BitLength) : nat
-      requires GetOctet(n) >= MinModulusOctets(padding)
+    function method MaxEncryptionBytes(padding : PaddingMode, modulusN : nat) : nat
+      requires GetOctet(modulusN) >= MinModulusOctets(padding)
     {
       match padding {
-        // mLen <= GetOctet(n) - 11
-        case PKCS1 => GetOctet(n) - 11
-        // Per  mLen <= GetOctet(n) - 2 * hashLengthBytes - 2
-        case OAEP_SHA1 => GetOctet(n) - 2 * SHA1_HASH_BYTES - 2
-        case OAEP_SHA256 => GetOctet(n) - 2 * SHA256_HASH_BYTES - 2
-        case OAEP_SHA384 => GetOctet(n) - 2 * SHA384_HASH_BYTES - 2
-        case OAEP_SHA512 => GetOctet(n) - 2 * SHA512_HASH_BYTES - 2
+        // mLen <= k - 11
+        case PKCS1 => GetOctet(modulusN) - 11
+        // Per  mLen <= k - 2 * hashLengthBytes - 2
+        case OAEP_SHA1 => GetOctet(modulusN) - 2 * SHA1_HASH_BYTES - 2
+        case OAEP_SHA256 => GetOctet(modulusN) - 2 * SHA256_HASH_BYTES - 2
+        case OAEP_SHA384 => GetOctet(modulusN) - 2 * SHA384_HASH_BYTES - 2
+        case OAEP_SHA512 => GetOctet(modulusN) - 2 * SHA512_HASH_BYTES - 2
         }
     }
 
     class {:extern} RSA {
-      static method {:extern} GenerateKeyPair(bits : BitLength, padding: PaddingMode)
+      static method {:extern} GenerateKeyPair(strength : Strength, padding: PaddingMode)
           returns (publicKey : seq<uint8>, privateKey : seq<uint8>)
-        requires GetOctet(bits) >= MinModulusOctets(padding)
+        requires GetOctet(strength as nat) >= MinModulusOctets(padding)
 
       static method {:extern} Decrypt(padding : PaddingMode, privateKey : seq<uint8>, cipherText : seq<uint8>)
           returns (res : Result<seq<uint8>>)
